FoC/Book/Chapter02/Section04.lean
@@ -70,18 +70,13 @@ theorem injective_definition (f : alpha -> beta) :
     Fn.Injective f <-> forall {x y}, f x = f y -> x = y :=
   Iff.rfl
 
-theorem injective_iff_distinct_images (f : alpha -> beta) :
+theorem injective_iff_distinct_images [DecidableEq alpha] (f : alpha -> beta) :
     Fn.Injective f <-> forall x y, x ≠ y -> f x ≠ f y :=
   Fn.injective_iff_distinct_images f
 
 theorem distinct_images_of_injective {f : alpha -> beta}
     (hf : Fn.Injective f) : forall x y, x ≠ y -> f x ≠ f y :=
   Fn.distinct_images_of_injective hf
-
-theorem injective_iff_distinct_images_decidable [DecidableEq alpha]
-    (f : alpha -> beta) :
-    Fn.Injective f <-> forall x y, x ≠ y -> f x ≠ f y :=
-  Fn.injective_iff_distinct_images_decidable f
 
 theorem bijective_definition (f : alpha -> beta) :
     Fn.Bijective f <-> Fn.Injective f ∧ Fn.Surjective f :=
