FoC/Book/Chapter03/Section07.lean
@@ -133,13 +133,13 @@ theorem regular_languages_have_pumping_property {L : Language alpha}
     Pumping.HasPumpingProperty L :=
   Pumping.regular_hasPumpingProperty hL
 
-theorem dfa_pumping_length_decidable [DecidableEq state] (M : DFA alpha state) :
+theorem dfa_pumping_length [DecidableEq state] (M : DFA alpha state) :
     Pumping.PumpingLength (DFA.Language M) (M.statesFinite.elems.length + 1) :=
-  Pumping.dfa_pumpingLength_decidable M
+  Pumping.dfa_pumpingLength M
 
-theorem dfa_has_pumping_property_decidable [DecidableEq state] (M : DFA alpha state) :
+theorem dfa_has_pumping_property [DecidableEq state] (M : DFA alpha state) :
     Pumping.HasPumpingProperty (DFA.Language M) :=
-  Pumping.dfa_hasPumpingProperty_decidable M
+  Pumping.dfa_hasPumpingProperty M
 
 theorem pumping_lemma_conclusion (L : Language alpha) :
     Pumping.PumpingLemmaConclusion L :=
