FoC/Foundation/Relations.lean
@@ -115,16 +115,6 @@ theorem overlapping_classes_equal {R : Rel alpha} (h : Equivalence R)
       exact class_equal_of_related h hab
 
 theorem classes_equal_or_disjoint {R : Rel alpha} (h : Equivalence R)
-    (a b : alpha) :
-    FSet.Equal (Class R a) (Class R b) ∨ FSet.Disjoint (Class R a) (Class R b) := by
-  classical
-  by_cases hoverlap : exists x, x ∈ Class R a ∧ x ∈ Class R b
-  · exact Or.inl (overlapping_classes_equal h hoverlap)
-  · exact Or.inr (by
-      intro x hx
-      exact hoverlap (Exists.intro x hx))
-
-theorem classes_equal_or_disjoint_decidable {R : Rel alpha} (h : Equivalence R)
     (a b : alpha)
     [Decidable (exists x, x ∈ Class R a ∧ x ∈ Class R b)] :
     FSet.Equal (Class R a) (Class R b) ∨ FSet.Disjoint (Class R a) (Class R b) := by
